Bap_i386.v
@@ -17,8 +17,6 @@ Require Import NArith.
 Require Import Program.Equality.
 Require Import Structures.Equalities.
 
-(* Instantiation of BAP for the x86 architectures *)
-
 (* Variables found in IL code lifted from x86 native code: *)
 Inductive x86var :=
   (* Main memory: MemT 32 *)
@@ -66,7 +64,7 @@ Module X86Arch <: Architecture.
   Proof. discriminate 1. Qed.
 End X86Arch.
 
-(* Instantiate the BAP semantics modules with the x86 identifiers above. *)
+(* Instantiate the static semantics module with the x86 identifiers above. *)
 
 Module BAPx86 := BAPStatics X86Arch.
 Import BAPx86.
@@ -93,26 +91,431 @@ Definition x86_wtm {s v mem mw} := @models_wtm x86typctx s v mem mw.
 Definition x86_regsize {s v u w} := @models_regsize x86typctx s v u w.
 
 
+
+(* Create some automated machinery for simplifying symbolic expressions commonly arising
+   from x86 instruction operations.  Mostly this involves simplifying e mod 2^w whenever
+   e < 2^w. *)
+
+(* Define an abbreviation for x86's parity flag computation, which produces uncomfortably
+   large symbolic expressions. *)
+Definition parity n :=
+  N.lnot ((N.lxor
+    (N.shiftr (N.lxor (N.shiftr (N.lxor (N.shiftr n 4) n) 2)
+                      (N.lxor (N.shiftr n 4) n)) 1)
+    (N.lxor (N.shiftr (N.lxor (N.shiftr n 4) n) 2)
+            (N.lxor (N.shiftr n 4) n))) mod 2^1) 1.
+
+Lemma fold_parity: forall n,
+  N.lnot ((N.lxor
+    (N.shiftr (N.lxor (N.shiftr (N.lxor (N.shiftr n 4) n) 2)
+                      (N.lxor (N.shiftr n 4) n)) 1)
+    (N.lxor (N.shiftr (N.lxor (N.shiftr n 4) n) 2)
+            (N.lxor (N.shiftr n 4) n))) mod 2^1) 1
+  = parity n.
+Proof. intro. reflexivity. Qed.
+
+(* getmem assembles bytes into words by logical-or'ing them together, but sometimes it
+   is easier to reason about them as if they were added.  The following theorem proves
+   that logical-or and addition are the same when the operands share no common bits. *)
+Theorem lor_plus:
+  forall a b (A0: N.land a b = 0), N.lor a b = a + b.
+Proof.
+  destruct a as [|a]; destruct b as [|b]; intros; try reflexivity.
+  simpl in *. apply f_equal. revert b A0.
+  induction a; destruct b; simpl; intros; try solve [ reflexivity | discriminate A0 ].
+    destruct (Pos.land a b); discriminate A0.
+    all: rewrite IHa; [ reflexivity | destruct (Pos.land a b); [ reflexivity | discriminate A0 ]].
+Qed.
+
+(* ((width) memory[...]) mod 2^width = (width) memory[...] *)
+Lemma memlo: forall w1 w2 m a, welltyped_memory m -> w1 <= w2 ->
+  (getmem LittleE w1 m a) mod 2^w2 = getmem LittleE w1 m a.
+Proof.
+  intros. apply N.mod_small. eapply N.lt_le_trans.
+    apply getmem_bound. assumption.
+    apply N.pow_le_mono_r. discriminate 1. assumption.
+Qed.
+
+(* (e mod 2^b) mod 2^c = e mod 2^(min b c) *)
+Lemma dblmod_l: forall a b c, b <= c -> (a mod 2^b) mod 2^c = a mod 2^b.
+Proof.
+  intros. repeat rewrite <- N.land_ones.
+  rewrite <- N.land_assoc, (N.land_comm (N.ones _)), N.land_ones, N.ones_mod_pow2.
+  reflexivity. assumption.
+Qed.
+
+Lemma dblmod_r: forall a b c, c <= b -> (a mod 2^b) mod 2^c = a mod 2^c.
+Proof.
+  intros. repeat rewrite <- N.land_ones.
+  rewrite <- N.land_assoc, N.land_ones, N.ones_mod_pow2.
+  reflexivity. assumption.
+Qed.
+
+(* e & (N.ones w) = e mod 2^w *)
+Remark land_mod_r: forall x y z, N.log2 (N.succ y) = N.succ (N.log2 y) -> z = N.log2 (N.succ y) ->
+  N.land x y = x mod 2^z.
+Proof.
+  intros x y z H1 H2. subst z. destruct y.
+    rewrite N.mod_1_r. apply N.land_0_r.
+
+    apply N.log2_eq_succ_iff_pow2 in H1; [|reflexivity]. destruct H1 as [b H1].
+    rewrite H1, N.log2_pow2 by apply N.le_0_l.
+    rewrite <- (N.pred_succ (Npos p)), H1, <- N.ones_equiv.
+    apply N.land_ones.
+Qed.
+
+(* (a & b) ^ c = (a ^ c) & b whenever b & c = c *)
+Lemma lxor_land:
+  forall a b c, N.land b c = c -> N.lxor (N.land a b) c = N.land (N.lxor a c) b.
+Proof.
+ intros. apply N.bits_inj. apply N.bits_inj_iff in H. intro n. specialize (H n).
+ do 2 rewrite N.land_spec, N.lxor_spec. rewrite <- H, N.land_spec.
+ repeat destruct (N.testbit _ n); reflexivity.
+Qed.
+
+Remark land_mod_l: forall x y z, N.log2 (N.succ x) = N.succ (N.log2 x) -> z = N.log2 (N.succ x) ->
+  N.land x y = y mod 2^z.
+Proof. intros x y. rewrite N.land_comm. apply land_mod_r. Qed.
+
+(* (x*y) mod x = 0 *)
+Remark mod_mul_l: forall x y, x<>0 -> (x*y) mod x = 0.
+Proof. intros. rewrite N.mul_comm. apply N.mod_mul. assumption. Qed.
+
+(* (x+y) mod x = y mod x *)
+Remark mod_add_l: forall x y, x<>0 -> (x+y) mod x = y mod x.
+Proof. intros. rewrite <- N.add_mod_idemp_l, N.mod_same, N.add_0_l by assumption. reflexivity. Qed.
+
+(* (y+x) mod x = y mod x *)
+Remark mod_add_r: forall x y, y<>0 -> (x+y) mod y = x mod y.
+Proof. intros. rewrite <- N.add_mod_idemp_r, N.mod_same, N.add_0_r by assumption. reflexivity. Qed.
+
+(* (x*z + y) mod z = y mod z *)
+Remark mod_add_mul_lr: forall x y z, z<>0 -> (x*z + y) mod z = y mod z.
+Proof. intros. rewrite <- N.add_mod_idemp_l, N.mod_mul, N.add_0_l by assumption. reflexivity. Qed.
+
+(* (z*x + y) mod z = y mod z *)
+Remark mod_add_mul_ll: forall x y z, z<>0 -> (z*x + y) mod z = y mod z.
+Proof. intros. rewrite <- N.add_mod_idemp_l, mod_mul_l, N.add_0_l by assumption. reflexivity. Qed.
+
+(* (x + y*z) mod z = x mod z *)
+Remark mod_add_mul_rr: forall x y z, z<>0 -> (x + y*z) mod z = x mod z.
+Proof. intros. rewrite <- N.add_mod_idemp_r, N.mod_mul, N.add_0_r by assumption. reflexivity. Qed.
+
+(* (x + z*y) mod z = x mod z *)
+Remark mod_add_mul_rl: forall x y z, z<>0 -> (x + z*y) mod z = x mod z.
+Proof. intros. rewrite <- N.add_mod_idemp_r, mod_mul_l, N.add_0_r by assumption. reflexivity. Qed.
+
+(* (mem a) mod 2^8 = mem a *)
+Remark mem_small: forall m a, welltyped_memory m -> (m a) mod 2^Mb = m a.
+Proof. intros. apply N.mod_small, H. Qed.
+
+(* e << w = 0 whenever e < 2^w *)
+Lemma shiftr_low_pow2: forall a n, a < 2^n -> N.shiftr a n = 0.
+Proof.
+  intros. destruct a. apply N.shiftr_0_l.
+  apply N.shiftr_eq_0. apply N.log2_lt_pow2. reflexivity. assumption.
+Qed.
+
+
+Create HintDb mod_pow2 discriminated.
+Global Hint Rewrite N.sub_0_r : mod_pow2.
+Global Hint Rewrite N.add_0_l : mod_pow2.
+Global Hint Rewrite N.add_0_r : mod_pow2.
+Global Hint Rewrite N.mul_0_l : mod_pow2.
+Global Hint Rewrite N.mul_0_r : mod_pow2.
+Global Hint Rewrite N.land_0_l : mod_pow2.
+Global Hint Rewrite N.land_0_r : mod_pow2.
+Global Hint Rewrite N.lor_0_l : mod_pow2.
+Global Hint Rewrite N.lor_0_r : mod_pow2.
+Global Hint Rewrite N.lxor_0_l : mod_pow2.
+Global Hint Rewrite N.lxor_0_r : mod_pow2.
+Global Hint Rewrite getmem_Mb : mod_pow2.
+Global Hint Rewrite N.mul_1_l : mod_pow2.
+Global Hint Rewrite N.mul_1_r : mod_pow2.
+Global Hint Rewrite fold_parity : mod_pow2.
+Global Hint Rewrite N.lxor_nilpotent : mod_pow2.
+Global Hint Rewrite N.mod_same using discriminate 1 : mod_pow2.
+Global Hint Rewrite N.mod_mul using discriminate 1 : mod_pow2.
+Global Hint Rewrite lxor_land using reflexivity : mod_pow2.
+Global Hint Rewrite dblmod_l using discriminate 1 : mod_pow2.
+Global Hint Rewrite dblmod_r using discriminate 1 : mod_pow2.
+Global Hint Rewrite mod_mul_l using discriminate 1 : mod_pow2.
+Global Hint Rewrite mod_add_l using discriminate 1 : mod_pow2.
+Global Hint Rewrite mod_add_r using discriminate 1 : mod_pow2.
+Global Hint Rewrite mod_add_mul_lr using discriminate 1 : mod_pow2.
+Global Hint Rewrite mod_add_mul_ll using discriminate 1 : mod_pow2.
+Global Hint Rewrite mod_add_mul_rr using discriminate 1 : mod_pow2.
+Global Hint Rewrite mod_add_mul_rl using discriminate 1 : mod_pow2.
+Global Hint Rewrite mem_small using assumption : mod_pow2.
+(*
+Global Hint Rewrite memlo using solve [ discriminate 1 | assumption ] : mod_pow2.
+Global Hint Rewrite shiftr_low_pow2 using solve_lt : mod_pow2.
+Global Hint Rewrite N.mod_small using solve_lt : mod_pow2.
+*)
+
+
+(* When reducing modulo operations, try auto-solving inequalities of the form x < 2^w. *)
+
+Lemma lnot_bound: forall x y, x < 2^y -> N.lnot x y < 2^y.
+Proof.
+  intros. apply hibits_zero_bound. intros.
+  rewrite N.lnot_spec_high by assumption.
+  eapply bound_hibits_zero; eassumption.
+Qed.
+
+Lemma lxor_bound: forall x y z, x < 2^z -> y < 2^z -> N.lxor x y < 2^z.
+Proof.
+  intros. apply logic_op_bound; [| assumption .. ].
+  intros. rewrite N.lxor_spec, Z1, Z2. reflexivity.
+Qed.
+
+Lemma land_bound: forall x y z, x < 2^z -> y < 2^z -> N.land x y < 2^z.
+Proof.
+  intros. apply logic_op_bound; [| assumption .. ].
+  intros. rewrite N.land_spec, Z1, Z2. reflexivity.
+Qed.
+
+Lemma lor_bound: forall x y z, x < 2^z -> y < 2^z -> N.lor x y < 2^z.
+Proof.
+  intros. apply logic_op_bound; [|assumption .. ].
+  intros. rewrite N.lor_spec, Z1, Z2. reflexivity.
+Qed.
+
+Ltac solve_lt_prim :=
+  reflexivity +
+  eassumption +
+  (apply N.mod_upper_bound; discriminate 1) +
+  lazymatch goal with [ M: models x86typctx ?s, R: ?s ?r = Some (VaN (?x,?w)) |- ?x < _ ] => apply (x86_regsize M R)
+                    | [ WTM: welltyped_memory ?m |- ?m _ < _ ] => apply WTM end +
+  (apply getmem_bound; assumption) +
+  (apply lxor_bound; solve_lt) +
+  (apply land_bound; solve_lt) +
+  (apply lor_bound; solve_lt) +
+  (apply lnot_bound; solve_lt) +
+  (eapply N.le_lt_trans; [ apply N.le_sub_l | solve_lt ])
+with solve_lt :=
+  solve_lt_prim +
+  (eapply N.lt_le_trans; [ solve_lt_prim | discriminate 1 ]).
+
+(* Try to auto-simplify modular arithmetic expressions within a Coq expression resulting from
+   functional interpretation of an x86 IL statement.
+
+   Implementation notes:  Currently I am using a combination of autorewrite and repeated
+   context-matching for this, since it's the fastest solution I can find (as of Coq 8.0).
+   Using rewrite_strat with topdown strategy is much slower; I'm not sure why. *)
+
+Tactic Notation "simpl_x86" "in" hyp(H) :=
+  autorewrite with mod_pow2 in H;
+  repeat (match type of H with
+  | context [ (getmem LittleE ?w1 ?m ?a) mod 2^?w2 ] => rewrite (memlo w1 w2 m a) in H; [| assumption | discriminate 1 ]
+  | context [ N.shiftr ?X ?Y ] => rewrite (shiftr_low_pow2 X Y) in H by solve_lt
+  | context [ ?X mod ?M ] => rewrite (N.mod_small X M) in H by solve_lt
+  | context [ N.land ?X ?Y ] => (erewrite (land_mod_r X Y) in H +
+                                 erewrite (land_mod_l X Y) in H); [| reflexivity | simpl;reflexivity ]
+  end; autorewrite with mod_pow2 in H).
+
+Ltac simpl_x86 :=
+  autorewrite with mod_pow2;
+  repeat (match goal with
+  | |- context [ (getmem LittleE ?w1 ?m ?a) mod 2^?w2 ] => rewrite (memlo w1 w2 m a); [| assumption | discriminate 1 ]
+  | |- context [ N.shiftr ?X ?Y ] => rewrite (shiftr_low_pow2 X Y) by solve_lt
+  | |- context [ ?X mod ?M ] => rewrite (N.mod_small X M) by solve_lt
+  | |- context [ N.land ?X ?Y ] => (erewrite (land_mod_r X Y) +
+                                    erewrite (land_mod_l X Y)); [| reflexivity | simpl;reflexivity ]
+  end; autorewrite with mod_pow2).
+
+
+
+(* Introduce automated machinery for verifying an x86 machine code subroutine (or collection
+   of subroutines) by (1) defining a set of Floyd-Hoare invariants (including pre- and post-
+   conditions) and (2) proving that symbolically executing the program starting at any
+   invariant point in a state that satisfies the program until the next invariant point always
+   yields a state that satisfies the reached invariant.  This proves partial correctness of
+   the subroutine.
+
+   In order for this methodology to prove that a post-condition holds at subroutine exit,
+   we must attach one of these invariants (the post-condition) to the return address of the
+   subroutine.  This is a somewhat delicate process, since unlike all the other code addresses,
+   the exact value of the return address is not known until runtime.  We therefore adopt the
+   following conventions:  Assume that an x86 subroutine begins with a return address located
+   at a particular memory address (determined by the subroutine's calling convention).  The
+   subroutine "exits" when control flows to that address.  As a precondition of the subroutine,
+   we assume that the subroutine program p does not assign an IL block to the return address
+   (i.e., p retaddr = None).  If this assumption is violated, it means that the caller is
+   part of the subroutine (i.e., the subroutine recursively called itself), which is not
+   really the end of the subroutine's execution. *)
+
+
+(* A subroutine invariant takes a program p, a set of invariants inv_set assigned to various
+   fixed code addresses, a post-condition (postcond), and a return address retaddr (which is
+   usually a symbolic Coq expression that extracts the appropriate value from memory), and
+   uses those to map each exit condition, store, and step count to a proposition.
+   Implementation note: Program p is not actually used in the definition, but including it in
+   the parameters helps Coq more easily unify some of the goals in the automated machinery
+   that follows. *)
+
+Definition x86_subroutine_inv (p:program) inv_set postcond retaddr x (s:store) (n:nat) : option Prop :=
+  match x with
+  | Exit a => if N.eq_dec a retaddr then Some (postcond a x s n) else inv_set a x s n
+  | _ => Some True
+  end.
+
+(* Since we are proving partial correctness, we know that the computation doesn't get aborted
+   by a computation limit in the middle (since that violates the termination assumption). *)
+Remark not_unfinished:
+  forall x (a':addr) RW p a s m n s' x',
+  match x with
+  | Some (Exit a2) => exec_prog RW p a2 s m n s' x'
+  | None => exec_prog RW p a s m n s' x'
+  | Some x2 => Exit a' = x2
+  end -> x <> Some Unfinished.
+Proof. intros. destruct x as [e|]; [destruct e|]; discriminate. Qed.
+
+(* If we reach the return address during symbolic interpretation, stop and request that the
+   user prove the post-condition using the current state. *)
+Remark x86_returning:
+  forall ra s n inv_set (postcond: addr -> exit -> store -> nat -> Prop) p RW m n' s' x',
+  postcond ra (Exit ra) s n ->
+  next_inv_sat (x86_subroutine_inv p inv_set postcond ra)
+               match x86_subroutine_inv p inv_set postcond ra (Exit ra) s n with
+               | Some _ => true | None => false end
+               (Exit ra) RW p s m n n' s' x'.
+Proof.
+  intros. unfold x86_subroutine_inv. destruct (N.eq_dec ra ra) eqn:H'.
+    apply NISHere. rewrite H'. assumption.
+    exfalso. apply n0. reflexivity.
+Qed.
+
+(* If we reach some other address to which an invariant has been assigned, top and request
+   that the user prove the invariant using the current state. *)
+Remark x86_not_returning_invhere (P: Prop):
+  forall p inv_set postcond ra a s n
+         (RET: p ra = match p a with Some _ => None | None => Some (0,Nop) end)
+         (IS: inv_set a (Exit a) s n = Some P),
+  P ->
+  match x86_subroutine_inv p inv_set postcond ra (Exit a) s n with Some P => P | None => False end.
+Proof.
+  intros. unfold x86_subroutine_inv. destruct (N.eq_dec a ra) as [EQ|NE].
+    subst a. destruct (p ra); discriminate RET.
+    rewrite IS. assumption.
+Qed.
+
+(* If we're at a code address to which no invariant has been assigned, step the
+   computation to the next instruction. *)
+Remark x86_not_returning_invstep (b:bool):
+  forall OP inv_set postcond a ra s n RW p m n' s' x'
+         (RET: p ra = match p a with Some _ => None | None => Some (0,Nop) end)
+         (IS: match inv_set a (Exit a) s n with Some _ => true | None => false end = b),
+  next_inv_sat OP b (Exit a) RW p s m n n' s' x' ->
+  next_inv_sat OP match x86_subroutine_inv p inv_set postcond ra (Exit a) s n with
+                  | Some _ => true | None => false end
+                  (Exit a) RW p s m n n' s' x'.
+Proof.
+  intros.
+  unfold x86_subroutine_inv. destruct (N.eq_dec a _) as [EQ|NE].
+    rewrite <- EQ in RET. destruct (p a); discriminate RET.
+    rewrite IS. exact H.
+Qed.
+
+(* Some versions of Coq check injection-heavy proofs very slowly (at Qed).  This slow-down can
+   be avoided by sequestering prevalent injections into lemmas, as we do here. *)
+Remark inj_prog_stmt: forall (sz1 sz2: N) (q1 q2: stmt),
+                      Some (sz1,q1) = Some (sz2,q2) -> sz1=sz2 /\ q1=q2.
+Proof. injection 1 as. split; assumption. Qed.
+
+(* Values of IL temp variables are ignored by the x86 interpreter once the IL block that
+   generated them completes.  We can therefore generalize them away at IL block boundaries
+   to simplify the expression. *)
+Ltac generalize_temps :=
+  repeat match goal with |- context c [ update vareq ?S (V_TEMP ?N) (Some ?U) ] => lazymatch goal with |- ?G =>
+    let u := fresh "tmp" in
+      set (u:=Some U) in |- * at 0;
+      let c' := context c[update vareq S (V_TEMP N) u] in
+        change G with c'; generalize u; clear u; intro
+  end end.
+
+(* If asked to step the computation when we're already at an invariant point, just
+   make the proof goal be the invariant. *)
+Ltac x86_invhere := first
+  [ eapply NISHere, x86_not_returning_invhere; [assumption|reflexivity|simpl_stores]
+  | apply x86_returning ]; simpl_x86.
+
+(* Symbolically evaluate an x86 machine instruction for one step, and simplify the resulting
+   Coq expressions. *)
+Ltac x86_step_and_simplify XS XP' :=
+  (bsimpl in XS; [|exact XP']);
+  revert XS; generalize_temps; intro XS;
+  simpl_x86 in XS.
+
+(* If we're not at an invariant, symbolically interpret the program for one machine
+   language instruction.  (The user can use "do" to step through many instructions,
+   but often it is wiser to pause and do some manual simplification of the state at
+   various points.) *)
+Ltac x86_invseek :=
+  apply NISStep;
+  let sz := fresh "sz" in let q := fresh "Q" in let s := fresh "s" in let x := fresh "x" in
+  let LT := fresh "LT" in let IL := fresh "IL" in let XS := fresh "XS" in let XP' := fresh "XP'" in
+  intros sz q s x LT IL XS XP'; clear LT;
+  apply not_unfinished in XP';
+  apply inj_prog_stmt in IL; destruct IL; subst sz q;
+  lazymatch goal with |- context [ Exit (?x + ?y) ] => simpl (x+y) end;
+  x86_step_and_simplify XS XP';
+  repeat lazymatch goal with [ ACC: MemAcc _ _ _ _ _ _ |- _ ] => simpl_x86 ACC; revert ACC end; intros;
+  repeat lazymatch type of XS with exec_stmt _ _ (if ?c then _ else _) _ _ _ =>
+    let BC := fresh "BC" in
+    lazymatch c with (if ?c2 then _ else _) => destruct c2 eqn:BC
+                   | N.lnot (if ?c2 then _ else _) 1 => destruct c2 eqn:BC
+                   | _ => destruct c eqn:BC end;
+    simpl_x86 in BC;
+    x86_step_and_simplify XS XP'
+  end;
+  clear XP'; repeat match goal with [ u:value |- _ ] => clear u
+                                  | [ u:option value |- _ ] => clear u end;
+  lazymatch type of XS with s=_ /\ x=_ =>
+    destruct XS; subst x;
+    first [ apply (x86_not_returning_invstep false); [assumption|reflexivity|subst s]
+          | apply (x86_not_returning_invstep true); [assumption|reflexivity|subst s]
+          | apply x86_returning; subst s ]
+  end.
+
+(* Clear any stale memory-access hypotheses (arising from previous computation steps)
+   and either step to the next machine instruction (if we're not at an invariant) or
+   produce an invariant as a proof goal. *)
+Ltac x86_step :=
+  repeat match goal with [ H: MemAcc ?RW _ _ _ _ _ |- next_inv_sat _ _ _ ?RW _ _ _ _ _ _ _ ] => clear H end;
+  first [ x86_invseek; try x86_invhere | x86_invhere ].
+
+
 Module X86Notations.
 
-Notation "Ⓜ m" := (Some (VaM m 32)) (at level 20).
-Notation "ⓑ u" := (Some (VaN (u,1))) (at level 20).
-Notation "Ⓑ u" := (Some (VaN (u,8))) (at level 20).
-Notation "Ⓦ u" := (Some (VaN (u,16))) (at level 20).
-Notation "Ⓓ u" := (Some (VaN (u,32))) (at level 20).
-Notation "Ⓠ u" := (Some (VaN (u,64))) (at level 20).
-Notation "Ⓧ u" := (Some (VaN (u,128))) (at level 20).
-Notation "Ⓨ u" := (Some (VaN (u,256))) (at level 20).
-Notation "m [ a : w ]" := (getmem LittleE w m a) (at level 10).
-Notation "m [ a : w := v ]" := (setmem LittleE w m a v) (at level 10).
-Notation "x ⊕ y" := ((x+y) mod 2^32) (at level 50, left associativity).
-Notation "x ⊖ y" := ((x-y) mod 2^32) (at level 50, left associativity).
-Notation "x ⊗ y" := ((x*y) mod 2^32) (at level 40, left associativity).
-Notation "x << y" := (N.shiftl x y) (at level 40, left associativity).
-Notation "x >> y" := (N.shiftr x y) (at level 40, left associativity).
-Notation "x >>> y" := (ashiftr 32 x y) (at level 40, left associativity).
-Notation "x .& y" := (N.land x y) (at level 55, left associativity).
-Notation "x .| y" := (N.lor x y) (at level 55, left associativity).
-Notation "x .^ y" := (N.lxor x y) (at level 55, left associativity).
+Notation "Ⓜ m" := (Some (VaM m 32)) (at level 20). (* memory value *)
+Notation "ⓑ u" := (Some (VaN (u,1))) (at level 20). (* bit value *)
+Notation "Ⓑ u" := (Some (VaN (u,8))) (at level 20). (* byte value *)
+Notation "Ⓦ u" := (Some (VaN (u,16))) (at level 20). (* word value *)
+Notation "Ⓓ u" := (Some (VaN (u,32))) (at level 20). (* dword value *)
+Notation "Ⓠ u" := (Some (VaN (u,64))) (at level 20). (* quad word value *)
+Notation "Ⓧ u" := (Some (VaN (u,128))) (at level 20). (* xmm value *)
+Notation "Ⓨ u" := (Some (VaN (u,256))) (at level 20). (* ymm value *)
+Notation "m Ⓑ[ a ]" := (getmem LittleE 8 m a) (at level 10). (* read byte from memory *)
+Notation "m Ⓦ[ a ]" := (getmem LittleE 16 m a) (at level 10). (* read word from memory *)
+Notation "m Ⓓ[ a ]" := (getmem LittleE 32 m a) (at level 10). (* read dword from memory *)
+Notation "m Ⓠ[ a ]" := (getmem LittleE 64 m a) (at level 10). (* read quad word from memory *)
+Notation "m Ⓧ[ a ]" := (getmem LittleE 128 m a) (at level 10). (* read xmm from memory *)
+Notation "m Ⓨ[ a ]" := (getmem LittleE 256 m a) (at level 10). (* read ymm from memory *)
+Notation "m [Ⓑ a := v ]" := (setmem LittleE 8 m a v) (at level 50, left associativity). (* write byte to memory *)
+Notation "m [Ⓦ a := v ]" := (setmem LittleE 16 m a v) (at level 50, left associativity). (* write word to memory *)
+Notation "m [Ⓓ a := v ]" := (setmem LittleE 32 m a v) (at level 50, left associativity). (* write dword to memory *)
+Notation "m [Ⓠ a := v ]" := (setmem LittleE 64 m a v) (at level 50, left associativity). (* write quad word to memory *)
+Notation "m [Ⓧ a := v ]" := (setmem LittleE 128 m a v) (at level 50, left associativity). (* write xmm to memory *)
+Notation "m [Ⓨ a := v ]" := (setmem LittleE 256 m a v) (at level 50, left associativity). (* write ymm to memory *)
+Notation "x ⊕ y" := ((x+y) mod 2^32) (at level 50, left associativity). (* modular addition *)
+Notation "x ⊖ y" := ((x-y) mod 2^32) (at level 50, left associativity). (* modular subtraction *)
+Notation "x ⊗ y" := ((x*y) mod 2^32) (at level 40, left associativity). (* modular multiplication *)
+Notation "x << y" := (N.shiftl x y) (at level 40, left associativity). (* logical shift-left *)
+Notation "x >> y" := (N.shiftr x y) (at level 40, left associativity). (* logical shift-right *)
+Notation "x >>> y" := (ashiftr 32 x y) (at level 40, left associativity). (* arithmetic shift-right *)
+Notation "x .& y" := (N.land x y) (at level 55, left associativity). (* logical and *)
+Notation "x .^ y" := (N.lxor x y) (at level 55, left associativity). (* logical xor *)
+Notation "x .| y" := (N.lor x y) (at level 55, left associativity). (* logical or *)
 
 End X86Notations.
